RocqOfRust/revm/revm_interpreter/instructions/simulate/table.v
@@ -60,6 +60,7 @@ Require Import revm.revm_interpreter.instructions.simulate.block_info.blob_basef
 Require Import revm.revm_interpreter.instructions.simulate.block_info.block_number.
 Require Import revm.revm_interpreter.instructions.simulate.block_info.chainid.
 Require Import revm.revm_interpreter.instructions.simulate.block_info.coinbase.
+Require Import revm.revm_interpreter.instructions.simulate.block_info.difficulty.
 Require Import revm.revm_interpreter.instructions.simulate.block_info.gaslimit.
 Require Import revm.revm_interpreter.instructions.simulate.block_info.timestamp.
 Require Import revm.revm_interpreter.instructions.simulate.control.jump.
@@ -420,6 +421,17 @@ Module FragmentInstructionTable.
     Function1.t (InstructionContext.t H WIRE WIRE_types) unit :=
     Function1.of_run
       (fun context => run_blob_basefee run_types run_host context).
+
+  Definition difficulty_function
+      {WIRE H : Set} `{Link WIRE} `{Link H}
+      {WIRE_types : InterpreterTypes.Types.t}
+      `{InterpreterTypes.Types.AreLinks WIRE_types}
+      {H_types : Host.Types.t} `{Host.Types.AreLinks H_types}
+      (run_types : InterpreterTypes.Run WIRE WIRE_types)
+      (run_host : Host.Run H H_types) :
+    Function1.t (InstructionContext.t H WIRE WIRE_types) unit :=
+    Function1.of_run
+      (fun context => run_difficulty run_types run_host context).
   Definition coinbase_function
       {WIRE H : Set} `{Link WIRE} `{Link H}
       {WIRE_types : InterpreterTypes.Types.t}
@@ -900,7 +912,10 @@ Module FragmentInstructionTable.
                   (ArrayPair.Build_t pop_instruction tail_after_pop)))))) in
     let tail_after_number :
         ArrayPairs.t (Instruction.t WIRE H WIRE_types) 188 :=
-      ArrayPair.Build_t unknown_instruction
+      ArrayPair.Build_t
+        {| Instruction.fn_ := difficulty_function
+             run_InterpreterTypes_for_WIRE run_host;
+           Instruction.static_gas := {| Integer.value := 2 |} |}
         (ArrayPair.Build_t
           {| Instruction.fn_ := gaslimit_function
                run_InterpreterTypes_for_WIRE run_host;
